Add NCFSC constraint into Consistency.

Coq/src/Consistency.v
@@ -105,8 +105,14 @@ Definition eco (m : model) : relation eventid :=
 
 (* sc order *)
 
-Definition psc (m : model) : relation eventid :=
-  ⦗ Sc ⦘ ⨾ hb ⨾ eco m ⨾ hb ⨾ ⦗ Sc ⦘.
+Definition psc_f (m : model) : relation eventid :=
+  ⦗F ∩₁ Sc⦘ ⨾ hb ⨾ (eco m ⨾ hb)^? ⨾ ⦗F ∩₁ Sc⦘.
+
+Definition scb :=
+  sb ∪ (sb \ same_loc) ⨾ hb ⨾ (sb \ same_loc) ∪ hb ∩ same_loc ∪ co ∪ fr.
+
+Definition psc_base :=
+  ⦗Sc⦘ ⨾ (⦗F⦘ ⨾ hb)^? ⨾ scb ⨾ (hb ⨾ ⦗F⦘)^? ⨾ ⦗Sc⦘.
 
 Record es_consistent {m} :=
   { ecf_irf : irreflexive ecf;
@@ -116,6 +122,7 @@ Record es_consistent {m} :=
 
     (* icf_R : dom_rel icf ⊆₁ R; *)
     (* icf_jf : irreflexive (jf ⨾ icf ⨾ jf⁻¹ ⨾ ew); *)
+    ncf_sc : acyclic (psc_f m ∪ psc_base)
   }.
 
 Record good_restriction (A : eventid -> Prop) := 
